Memory.thy
@@ -43,6 +43,7 @@ lemma memory_\<alpha>_set_stack[simp]:
   by (cases a'; fastforce)
   done
 
+
 lemma single_memory_\<alpha>_allocate[single_memory_simps]:
   assumes "a \<noteq> length m"
   shows "single_memory_\<alpha> (m@[mem_unset]) a = (single_memory_\<alpha> m) a"
@@ -106,20 +107,27 @@ lemma memory_\<alpha>_not_none_iff[simp]:
   by (cases s; cases a; simp add: single_memory_simps)
 
 
-lemma single_memory_\<alpha>_some_some_iff[single_memory_simps]:
-  "single_memory_\<alpha> s a = Some (Some v) \<longleftrightarrow> valid_single_memory_address s a \<and> s!a = mem_val v"
-  unfolding get_single_memory_def single_memory_\<alpha>_def valid_single_memory_address_def
-  by (cases "s!a"; simp)
+lemma memory_\<alpha>_allocate_validity[simp]:
+  assumes "memory_\<alpha> m' = (memory_\<alpha> m)(a := Some None)"
+  assumes "a \<noteq> a'"
+  shows "valid_memory_address m a' = valid_memory_address m' a' \<and> valid_memory_address m' a"
+  using assms
+  by simp
 
-lemma memory_\<alpha>_some_some_iff_heap[simp]:
-  "memory_\<alpha> (r,s,h) (haddr a) = Some (Some v) \<longleftrightarrow> valid_memory_address (r,s,h) (haddr a) \<and> h!a = mem_val v"
-  using single_memory_simps
-  by fastforce
+lemma memory_\<alpha>_set_validity[simp]:
+  assumes "memory_\<alpha> m' = (memory_\<alpha> m)(a := Some (Some v))"
+  assumes "memory_\<alpha> m a \<noteq> None"
+  shows "valid_memory_address m = valid_memory_address m'"
+  using assms
+  by (simp add: fun_eq_iff)
 
-lemma single_memory_\<alpha>_some_some_iff_stack[simp]:
-  "memory_\<alpha> (r,s,h) (saddr a) = Some (Some v) \<longleftrightarrow> valid_memory_address (r,s,h) (saddr a) \<and> s!a = mem_val v"
-  using single_memory_simps
-  by fastforce
+lemma memory_\<alpha>_free_validity[simp]:
+  assumes "memory_\<alpha> m' = (memory_\<alpha> m)(a := None)"
+  assumes "a \<noteq> a'"
+  shows "valid_memory_address m a' = valid_memory_address m' a' \<and> \<not>valid_memory_address m' a"
+  using assms
+  by simp
+
 
 
 section "Intro rules"
@@ -133,7 +141,7 @@ lemma wp_case_memory_value_intro[wp_intro]:
   by (cases x; simp)
 
 
-lemma wp_get_single_memory[THEN consequence, single_memory_intro]:
+lemma wp_get_single_memory_intro[THEN consequence, single_memory_intro]:
   assumes "single_memory_\<alpha> s a \<noteq> None"
   assumes "single_memory_\<alpha> s a \<noteq> Some None"
   shows "wp (get_single_memory s a) (\<lambda>x. single_memory_\<alpha> s a = Some (Some x))"
@@ -149,7 +157,7 @@ lemma wp_get_memory_intro[THEN consequence, wp_intro]:
   by (cases a; cases s; simp; intro single_memory_intro; simp)
 
 
-lemma wp_set_single_memory[THEN consequence, single_memory_intro]:
+lemma wp_set_single_memory_intro[THEN consequence, single_memory_intro]:
   assumes "single_memory_\<alpha> m a \<noteq> None"
   shows "wp (set_single_memory m a v) (\<lambda>m'. single_memory_\<alpha> m' = (single_memory_\<alpha> m)(a := Some (Some v)))"
   using assms
@@ -162,10 +170,10 @@ lemma wp_set_memory_intro[THEN consequence, wp_intro]:
   using assms 
   apply (cases a; cases s; simp)
   unfolding set_single_memory_def
-  by (intro wp_intro; simp add: single_memory_simps)+
+  by (intro wp_intro; simp add: single_memory_simps; rule ext; simp)+
 
 
-lemma wp_free_single_memory[THEN consequence, single_memory_intro]:
+lemma wp_free_single_memory_intro[THEN consequence, single_memory_intro]:
   assumes "single_memory_\<alpha> s a \<noteq> None"
   shows "wp (free_single_memory s a) (\<lambda>s'. (single_memory_\<alpha> s') = (single_memory_\<alpha> s)(a := None))"
   using assms
@@ -192,177 +200,13 @@ lemma wp_allocate_single_memory[THEN consequence, single_memory_intro]:
   by (intro wp_intro; auto simp: single_memory_simps)
 
 lemma wp_allocate_heap_intro[THEN consequence, wp_intro]:
-  "wp (return (allocate_heap s)) (\<lambda>(s', a). (memory_\<alpha> s') = (memory_\<alpha> s)(a := Some None) \<and> register_\<alpha> s = register_\<alpha> s')"
+  "wp (return (allocate_heap s)) (\<lambda>(s', a). (\<exists>a'. a = haddr a') \<and> (memory_\<alpha> s') = (memory_\<alpha> s)(a := Some None) \<and> register_\<alpha> s = register_\<alpha> s')"
   unfolding allocate_heap_def allocate_single_memory_def
   by (cases s; intro wp_intro; auto)
 
 lemma wp_allocate_stack_intro[THEN consequence, wp_intro]:
-  "wp (return (allocate_stack s)) (\<lambda>(s', a). (memory_\<alpha> s') = (memory_\<alpha> s)(a := Some None) \<and> register_\<alpha> s = register_\<alpha> s')"
+  "wp (return (allocate_stack s)) (\<lambda>(s', a). (\<exists>a'. a = saddr a') \<and> (memory_\<alpha> s') = (memory_\<alpha> s)(a := Some None) \<and> register_\<alpha> s = register_\<alpha> s')"
   unfolding allocate_stack_def allocate_single_memory_def
   by (cases s; intro wp_intro; auto)
-
-subsection "Simps"
-
-lemma memory_set_ok_iff[simp]: "valid_single_memory_address m a \<longleftrightarrow> (\<exists>m'. set_single_memory m a v = ok m')"
-  unfolding set_single_memory_def
-  by simp
-
-lemma memory_get_ok_iff[simp]: "valid_single_memory_address m a \<and> m!a \<noteq> mem_unset \<longleftrightarrow> (\<exists>v. get_single_memory m a = ok v)"
-  unfolding get_single_memory_def valid_single_memory_address_def
-  by (cases "m!a"; simp)
-
-
-subsection "Empty"
-
-lemma memory_empty_get: "get_single_memory empty_memory_model a = err unallocated_address"
-  unfolding empty_memory_model_def get_single_memory_def valid_single_memory_address_def
-  by simp
-
-lemma memory_empty_invalid: "\<not>valid_single_memory_address empty_memory_model a"
-  unfolding empty_memory_model_def valid_single_memory_address_def
-  by simp
-
-lemma memory_empty_set: "set_single_memory empty_memory_model a v = err unallocated_address"
-  unfolding empty_memory_model_def set_single_memory_def valid_single_memory_address_def
-  by simp
-
-
-subsection "Allocate"
-
-lemma memory_allocate_validity: "allocate_single_memory m = (m', i) \<Longrightarrow> \<not>valid_single_memory_address m i \<and> valid_single_memory_address m' i"
-  unfolding allocate_single_memory_def valid_single_memory_address_def
-  by auto
-
-lemma memory_allocate_independent_valid[simp]: "allocate_single_memory m = (m', a') \<Longrightarrow> a \<noteq> a' \<Longrightarrow> valid_single_memory_address m a \<longleftrightarrow> valid_single_memory_address m' a"
-  unfolding valid_single_memory_address_def allocate_single_memory_def
-  using nth_append_left
-  by fastforce
-
-lemma memory_allocate_independent_get: "allocate_single_memory m = (m', a') \<Longrightarrow> a \<noteq> a' \<Longrightarrow> get_single_memory m a = get_single_memory m' a" 
-  unfolding valid_single_memory_address_def allocate_single_memory_def get_single_memory_def
-  using nth_append_left
-  by (cases "a < a'"; fastforce)
-
-lemma memory_allocate_get_uninitialized: "allocate_single_memory m = (m', a) \<Longrightarrow> get_single_memory m' a = err uninitialized_address"
-  unfolding get_single_memory_def valid_single_memory_address_def allocate_single_memory_def
-  by auto
-
-
-subsection "Set"
-
-lemma memory_set_invalid: "\<not>valid_single_memory_address m a \<Longrightarrow> set_single_memory m a v = err unallocated_address"
-  unfolding set_single_memory_def
-  by simp
-
-lemma memory_set_ok_valid: "set_single_memory m a v = ok m' \<Longrightarrow> valid_single_memory_address m' a \<and> valid_single_memory_address m a"
-  unfolding set_single_memory_def
-  apply simp
-  unfolding valid_single_memory_address_def
-  by auto
-
-lemma wp_set_single_memory_independent_validity[THEN consequence, single_memory_intro]:
-  assumes "valid_single_memory_address m a"
-  shows "wp (set_single_memory m a v) (\<lambda> m'. valid_single_memory_address m' = valid_single_memory_address m)"
-  using assms
-  by (intro single_memory_intro; simp add: fun_eq_iff single_memory_simps)
-
-lemma wp_set_memory_independent_validity:
-  assumes "valid_memory_address s a"
-  shows "wp (set_memory s a v) (\<lambda> s'. valid_memory_address s' = valid_memory_address s)"
-  using assms
-  by (intro wp_intro; simp add: fun_eq_iff)
-
-lemma memory_set_override:
-  assumes "set_single_memory m i v = ok m'"
-  assumes "set_single_memory m' i v' = ok m''"
-  shows "get_single_memory m'' i = ok v'"
-  using assms
-  unfolding set_single_memory_def get_single_memory_def valid_single_memory_address_def
-  by auto
-
-lemma memory_set_override_wlp:
-  "wlp (do {
-    m' \<leftarrow> set_single_memory m a v1;
-    m'' \<leftarrow> set_single_memory m' a v2;
-    get_single_memory m'' a}) (\<lambda>v. v = v2)"
-  unfolding set_single_memory_def get_single_memory_def valid_single_memory_address_def
-  by (intro wp_intro; simp)
-
-
-lemma memory_set_identity: "get_single_memory m i = ok v \<Longrightarrow> set_single_memory m i v = ok m' \<Longrightarrow> m = m'"
-  unfolding get_single_memory_def set_single_memory_def
-  apply simp
-  unfolding valid_single_memory_address_def
-  apply (cases "m!i"; simp)
-  using list_update_id
-  by metis
-
-lemma memory_set_identity_wlp: "wlp (do { v \<leftarrow> get_single_memory m a; set_single_memory m a v }) ((=) m)"
-  unfolding get_single_memory_def set_single_memory_def valid_single_memory_address_def
-  apply (intro wp_intro; simp)
-  apply (cases "m!a"; simp)
-  using list_update_id
-  by metis
-
-
-lemma memory_set_get: "set_single_memory m i v = ok m' \<Longrightarrow> get_single_memory m' i = ok v"
-  unfolding get_single_memory_def set_single_memory_def valid_single_memory_address_def
-  by auto
-
-lemma memory_set_get_wlp: "wlp (do {m' \<leftarrow> set_single_memory m a v; get_single_memory m' a}) ((=) v)"
-  unfolding get_single_memory_def set_single_memory_def valid_single_memory_address_def
-  by (intro wp_intro; simp)
-
-
-lemma memory_set_independent_get: "set_single_memory m a' v = ok m' \<Longrightarrow> a \<noteq> a' \<Longrightarrow> get_single_memory m a = get_single_memory m' a"
-  unfolding get_single_memory_def set_single_memory_def
-  apply simp
-  unfolding valid_single_memory_address_def
-  by auto
-
-lemma memory_set_independent_get_wlp: "a \<noteq> a' \<Longrightarrow> wlp (set_single_memory m a' v) (\<lambda>m'. get_single_memory m' a = get_single_memory m a)"
-  unfolding get_single_memory_def set_single_memory_def
-  apply (intro wp_intro)
-  apply simp
-  unfolding valid_single_memory_address_def
-  by auto
-
-
-lemma memory_set_independent_valid: "set_single_memory m a' v = ok m' \<Longrightarrow> a \<noteq> a' \<Longrightarrow> valid_single_memory_address m a = valid_single_memory_address m' a"
-  unfolding get_single_memory_def set_single_memory_def
-  apply simp
-  unfolding valid_single_memory_address_def
-  by auto
-
-
-subsection "Get"
-
-lemma memory_get_ok_valid: "get_single_memory m a = ok v \<Longrightarrow> valid_single_memory_address m a"
-  unfolding get_single_memory_def
-  by simp
-
-
-subsection "Free"
-
-lemma memory_free_get: "free_single_memory m a = ok m' \<Longrightarrow> get_single_memory m' a = err unallocated_address"
-  unfolding free_single_memory_def get_single_memory_def valid_single_memory_address_def
-  by auto
-
-lemma memory_free_set: "free_single_memory m a = ok m' \<Longrightarrow> set_single_memory m' a v = err unallocated_address"
-  unfolding free_single_memory_def set_single_memory_def valid_single_memory_address_def
-  by auto
-
-lemma memory_free_invalid: "free_single_memory m a = ok m' \<Longrightarrow> \<not>valid_single_memory_address m' a \<and> valid_single_memory_address m a"
-  unfolding free_single_memory_def valid_single_memory_address_def
-  by auto
-
-lemma memory_free_independent_valid: "free_single_memory m a' = ok m' \<Longrightarrow> a \<noteq> a' \<Longrightarrow> valid_single_memory_address m a \<longleftrightarrow> valid_single_memory_address m' a"
-  unfolding free_single_memory_def valid_single_memory_address_def
-  by auto
-
-lemma memory_free_independent_get: "free_single_memory m a' = ok m' \<Longrightarrow> a \<noteq> a' \<Longrightarrow> get_single_memory m a = ok v \<longleftrightarrow> get_single_memory m' a = ok v"
-  unfolding free_single_memory_def get_single_memory_def valid_single_memory_address_def
-  by auto
-
 
 end
